cedar-lean/Cedar/Thm/Validation/Levels/BinaryApp.lean
@@ -51,15 +51,14 @@ theorem level_based_slicing_is_sound_inₑ {e₁ : Expr} {euid₁ euid₂ : Enti
   (hc : CapabilitiesInvariant c₀ request entities)
   (hr : RequestAndEntitiesMatchEnvironment env request entities)
   (ht : typeOf e₁ c₀ env = Except.ok (tx₁, c₁))
-  (hl : TypedExpr.EntityAccessAtLevel tx₁ n (n + 1))
-  (hel : ¬ TypedExpr.EntityLitViaPath tx₁ [])
+  (hl : TypedExpr.EntityAccessAtLevel tx₁ n (n + 1) [])
   (he : evaluate e₁ request entities = .ok (Value.prim (Prim.entityUID euid₁)))
   (hs : some slice = entities.sliceAtLevel request (n + 1))
   : inₑ euid₁ euid₂ entities = inₑ euid₁ euid₂ slice
 := by
   simp only [inₑ]
   cases heq : euid₁ == euid₂ <;> simp only [Bool.false_or, Bool.true_or]
-  have hfeq := checked_eval_entity_find_entities_eq_find_slice hc hr ht hl hel he hs
+  have hfeq := checked_eval_entity_find_entities_eq_find_slice hc hr ht hl he hs
   simp [hfeq, Entities.ancestorsOrEmpty]
 
 theorem level_based_slicing_is_sound_binary_app {op : BinaryOp} {e₁ e₂ : Expr} {n : Nat} {c₀ c₁: Capabilities} {env : Environment} {request : Request} {entities slice : Entities}
@@ -79,7 +78,7 @@ theorem level_based_slicing_is_sound_binary_app {op : BinaryOp} {e₁ e₂ : Exp
   case getTag hel hl₁ hl₂ | hasTag hel hl₁ hl₂ =>
     specialize ihe₂ hs hc hr htx₂ hl₂
     rw [←ihe₂]
-    have hl₁' := entity_access_at_level_then_at_level (by omega) hl₁
+    have hl₁' := entity_access_at_level_then_at_level hl₁
     specialize ihe₁ hs hc hr htx₁ hl₁'
     rw [←ihe₁]
     cases he₁ : evaluate e₁ request entities <;> simp only [Except.bind_ok, Except.bind_err]
@@ -89,12 +88,12 @@ theorem level_based_slicing_is_sound_binary_app {op : BinaryOp} {e₁ e₂ : Exp
     rename_i p₁ p₂
     cases p₁ <;> cases p₂ <;> simp only
     rename_i euid _
-    have hfeq := checked_eval_entity_find_entities_eq_find_slice hc hr htx₁ hl₁ hel he₁ hs
+    have hfeq := checked_eval_entity_find_entities_eq_find_slice hc hr htx₁ hl₁ he₁ hs
     simp only [hfeq, hasTag, getTag, Entities.tagsOrEmpty, Entities.tags, Map.findOrErr]
   case mem hel hl₁ hl₂ =>
     specialize ihe₂ hs hc hr htx₂ hl₂
     rw [←ihe₂]
-    have hl₁' := entity_access_at_level_then_at_level (by omega) hl₁
+    have hl₁' := entity_access_at_level_then_at_level hl₁
     specialize ihe₁ hs hc hr htx₁ hl₁'
     rw [←ihe₁]
     cases he₁ : evaluate e₁ request entities <;> simp only [Except.bind_ok, Except.bind_err]
@@ -104,11 +103,11 @@ theorem level_based_slicing_is_sound_binary_app {op : BinaryOp} {e₁ e₂ : Exp
     case prim =>
       rename_i p₁ p₂
       cases p₁ <;> cases p₂ <;> simp only
-      simp [level_based_slicing_is_sound_inₑ hc hr htx₁ hl₁ hel he₁ hs]
+      simp [level_based_slicing_is_sound_inₑ hc hr htx₁ hl₁ he₁ hs]
     case set =>
       rename_i p₁ sv
       cases p₁ <;> simp only
-      simp [inₛ, level_based_slicing_is_sound_inₑ hc hr htx₁ hl₁ hel he₁ hs]
+      simp [inₛ, level_based_slicing_is_sound_inₑ hc hr htx₁ hl₁ he₁ hs]
   case binaryApp hop hl₁ hl₂ =>
     specialize ihe₁ hs hc hr htx₁ hl₁
     specialize ihe₂ hs hc hr htx₂ hl₂
